# $$Lecture 3$$
$$rrison$$
## 2 叉乘的李代数性质
$X=\begin{bmatrix}
   x_1 \\\\
   x_2 \\\\
   x_3
  \end{bmatrix},
  Y=\begin{bmatrix}
   y_1 \\\\
   y_2 \\\\
   y_3
  \end{bmatrix},
  Z=\begin{bmatrix}
   z_1 \\\\
   z_2 \\\\
   z_3
  \end{bmatrix} \in V$
1. 封闭性 
$[X,Y]=\begin{bmatrix}
   x_2 y_3-x_3 y_2 \\\\
   x_3 y_1-x_1 y_3 \\\\
   x_1 y_2-x_2 y_1
  \end{bmatrix} \in V$
2. 双线性 
$[aX+bY,Z]$

$=\begin{bmatrix}
   a x_2 z_3 + b y_2 z_3 - a x_3 z_2 - b y_3 z_2 \\\\
   a x_3 z_1 + b y_3 z_1 - a x_1 z_3 - b y_1 z_3 \\\\
   a x_1 z_2 + b y_1 z_2 - a x_2 z_1 - b y_2 z_1
  \end{bmatrix}=\begin{bmatrix}
   a x_2 z_3- a x_3 z_2 \\\\
   a x_3 z_1 - a x_1 z_3 \\\\
   a x_1 z_2 - a x_2 z_1
  \end{bmatrix} + \begin{bmatrix}
   b y_2 z_3 - b y_3 z_2 \\\\
   b y_3 z_1 - b y_1 z_3 \\\\
   b y_1 z_2 - b y_2 z_1
  \end{bmatrix}$
  
  $= a\begin{bmatrix}
   x_2 z_3 - x_3 z_2 \\\\
   x_3 z_1 - x_1 z_3 \\\\
   x_1 z_2 - x_2 z_1
  \end{bmatrix} + b\begin{bmatrix}
   y_2 z_3 - y_3 z_2 \\\\
   y_3 z_1 - y_1 z_3 \\\\
   y_1 z_2 - y_2 z_1
  \end{bmatrix}
  =a[X,Z]+b[Y,Z]$
  
  $[Z,aX+bY]$
  
$=\begin{bmatrix}
   a x_3 z_2 + b y_3 z_2 - a x_2 z_3 - b y_2 z_3 \\\\
   a x_1 z_3 + b x_1 z_3 - a x_3 z_1 - b y_3 z_1 \\\\
   a x_2 z_1 + b y_2 z_1 - a x_1 z_2 - b y_1 z_2
  \end{bmatrix}=\begin{bmatrix}
   a x_3 z_2 - a x_2 z_3 \\\\
   a x_1 z_3  - a x_3 z_1 \\\\
   a x_2 z_1 - a x_1 z_2
  \end{bmatrix} + \begin{bmatrix}
   b y_3 z_2 - b y_2 z_3 \\\\
   b x_1 z_3 - b y_3 z_1 \\\\
   b y_2 z_1 - b y_1 z_2
  \end{bmatrix}$
  
  $= a\begin{bmatrix}
   x_3 z_2 - x_2 z_3 \\\\
   x_1 z_3  - x_3 z_1 \\\\
   x_2 z_1 - x_1 z_2
  \end{bmatrix} + b\begin{bmatrix}
   y_3 z_2 - y_2 z_3 \\\\
   x_1 z_3 - y_3 z_1 \\\\
   y_2 z_1 - y_1 z_2
  \end{bmatrix}
  =a[Z,X]+b[Z,Y]$
3. 自反性
$[X,X]=\begin{bmatrix}
   x_2 x_3-x_3 x_2 \\\\
   x_3 x_1-x_1 x_3 \\\\
   x_1 x_2-x_2 x_1
  \end{bmatrix}=\begin{bmatrix}
   0 \\\\
   0 \\\\
   0
  \end{bmatrix}$
4. 雅可比等价
$[X,[Y,Z]]+[Z,[X,Y]]+[Y,[Z,X]]$

$=\begin{bmatrix}
   x_2 (y_1 z_2 - y_2 z_1) - x_3 (y_3 z_1 - y_1 z_3) \\\\
   x_3 (y_2 z_3 - y_3 z_2) - x_1 (y_1 z_2 - y_2 z_1) \\\\
   x_1 (y_3 z_1 - y_1 z_3) - x_2 (y_2 z_3 - y_3 z_2)
  \end{bmatrix}+\begin{bmatrix}
   z_2 (x_1 y_2 - x_2 y_1) - z_3 (x_3 y_1 - x_1 y_3) \\\\
   z_3 (x_2 y_3 - x_3 y_2) - z_1 (x_1 y_2 - x_2 y_1) \\\\
   z_1 (x_3 y_1 - x_1 y_3) - z_2 (x_2 y_3 - x_3 y_2)
  \end{bmatrix}+\begin{bmatrix}
   y_2 (z_1 x_2 - z_2 x_1) - y_3 (z_3 x_1 - z_1 z_3) \\\\
   y_3 (z_2 x_3 - z_3 x_2) - y_1 (z_1 x_2 - z_2 x_1) \\\\
   y_1 (z_3 x_1 - z_1 x_3) - y_2 (z_2 x_3 - z_3 x_2)
  \end{bmatrix}$
  
  $=\begin{bmatrix}
   0 \\\\
   0 \\\\
   0
  \end{bmatrix}$
  
## 3 推导SE(3)指数映射
$e^{\xi^\wedge}=I+\begin{bmatrix}
   \phi^\wedge & \rho \\\\
   0 & 0
  \end{bmatrix}+\frac{1}{2!}\begin{bmatrix}
   \phi^\wedge & \rho \\\\
   0 & 0
  \end{bmatrix}+\frac{1}{3!}\begin{bmatrix}
   (\hat{\phi}\ \ )^2 & \hat{\phi}\ \ \rho \\\\
   0 & 0
  \end{bmatrix}+\dots=\begin{bmatrix}
   \sum_{n=0}^{\infty}\frac{1}{n!}(\hat{\phi}\ \ )^n & \sum_{n=0}^{\infty}\frac{1}{(n+1)!}(\hat{\phi}\ \ )^n\rho \\\\
   0^T & 1
  \end{bmatrix}$

  已知$$R=e^{\hat{\phi}}=\sum_{n=0}^{\infty}\frac{1}{n!}(\hat{\phi}\ \ )^n=cos\theta\cdot I+(1-cos\theta)aa^T+sin\theta\cdot\hat{a}\tag{1}$$
  
  令$J=\sum_{n=0}^{\infty}\frac{1}{(n+1)!}(\hat{\phi}\ \ )^n$, 
$J=I+\frac{1}{2!}\hat{\phi}\ +\frac{1}{3!}(\hat{\phi}\ )^2+\frac{1}{4!}(\hat{\phi}\ )^3+\frac{1}{5!}(\hat{\phi}\ )^4 + \dots$

$=aa^T-\hat{a}\ \hat{a}+\frac{1}{2!}\theta\hat{a}\ +\frac{1}{3!}\theta^2\hat{a}\ \hat{a}-\frac{1}{4!}\theta^3\hat{a}\ -\frac{1}{5!}\theta^4\hat{a}\ \hat{a} + \dots$

$=aa^T-\hat{a}\ \hat{a}\ (1-\frac{1}{3!}\theta^2+\frac{1}{5!}\theta^4+\dots)+\hat{a}\ (\frac{1}{2!}\theta-\frac{1}{4!}\theta^3+\dots)$

$=aa^T-\frac{1}{\theta}\hat{a}\ \hat{a}\ (\theta-\frac{1}{3!}\theta^3+\frac{1}{5!}\theta^5+\dots)+\frac{1}{\theta}\hat{a}\ (\frac{1}{2!}\theta^2-\frac{1}{4!}\theta^4+\dots)$

$=aa^T-\frac{sin\theta}{\theta}\hat{a}\ \hat{a}\ +\frac{1-cos\theta}{\theta}\hat{a}\ $

$=aa^T-\frac{sin\theta}{\theta}(aa^T-I)+\frac{1-cos\theta}{\theta}\hat{a}\ $

$=\frac{sin\theta}{\theta}I\ +(1-\frac{sin\theta}{\theta})aa^T+\frac{1-cos\theta}{\theta}\hat{a}\ $

then  $e^{\hat{\xi}}=\begin{bmatrix}
   \sum_{n=0}^{\infty}\frac{1}{n!}(\hat{\phi}\ \ )^n & \sum_{n=0}^{\infty}\frac{1}{(n+1)!}(\hat{\phi}\ \ )^n\rho \\\\
   0^T & 1
  \end{bmatrix}
  =\begin{bmatrix}
   R & J\rho \\\\
   0^T & 0
  \end{bmatrix}$,
where $R=cos\theta\cdot I+(1-cos\theta)aa^T+sin\theta\cdot\hat{a}\ \ , J=\frac{sin\theta}{\theta}I\ +(1-\frac{sin\theta}{\theta})aa^T+\frac{1-cos\theta}{\theta}\hat{a}\ $
## 4 伴随
证明$R\hat{a}\ \ R^T=(Ra\hat{)}$

$(Ra\hat{)}\ R=(Ra)\times R=(Ra)\times (RR^TR)=R(a\times (R^TR))=R(a\times I)=R\hat{a}$

$(Ra\hat{)}\ R=R\hat{a}$

$\rightarrow R\hat{a}\ R^T=(Ra\hat{)}\ $

已知$((Ra\hat{)}\ \ )^n=R\hat{a}\ R^T\cdot R\hat{a}\ R^T\cdot \dots \cdot R\hat{a}\ R^T=R(\hat{a}\ \ )^n R^T$
证明$SO(3)$伴随性质：
$Re^{\hat{p}}R^T=\sum_{n=0}^{\infty} R\frac{1}{n!}(\hat{p}\ )^n R^T=\sum_{n=0}^{\infty}\frac{1}{n!}((Rp\hat{)}\ \ )^n=e^{((Rp\hat{)}\ \ )^n}$
## 5 轨迹的描绘
见code/draw_trajectory.cpp
## 6 轨迹的误差
见code/draw_trajectory.cpp里面的CalcRMSE().

